finish proving the nested loop example

nested-loop.dfy
@@ -1,32 +1,37 @@
-﻿/**
- *  Challenge:
- *  Substitute a loop with valid invariants for the forall loop inside the main loop.
- */
-method foo(n: int)
+﻿method foo(n: nat)
 {
 	var mat := new bool[n,n];
-	forall i,j | (0 <= i < n && 0 <= j < n)
+	forall i,j | 0 <= i < n && 0 <= j < n
 	{
 		mat[i,j] := false;
 	}
 	var i := 0;
 	var j := 0;
 	while i < n
-		invariant 0 <= i <= n && 0 <= j <= n
-		invariant forall k, j :: 0 <= k < i && 0 <= j < n ==> mat[k,j];
+		invariant 0 <= i <= n
+		invariant forall k :: 0 <= k < i ==> INV(mat, k)
+		// The following invariant is syntactically equivalent 
+		// to the above one but cannot be verified.
+		// invariant forall k,j :: 0 <= k < i ==> 0 <= j < n ==> mat[k,j];
 	{
-		forall j: int | 0 <= j < n { mat[i,j] := true; }
-		/*
-		Cannot verify the following loop:
+		// In the latest version of Dafny (after Jan 2016), a forall loop 
+		// no longer implies its equivalent forall assertion trivially:
+		//		forall j | 0 <= j < n { mat[i,j] := true; }
+		//		assert forall j :: 0 <= j < n ==> mat[i,j]; //FAILED!
+		j := 0;
 		while j < n
-			invariant 0 <= i <= n && 0 <= j <= n
-			invariant forall i, j :: 0 <= i < i && 0 <= j < j ==> mat[i,j];
+			invariant j <= n;
+			invariant forall k :: 0 <= k < j ==> mat[i,k];
 		{
 			mat[i,j] := true;
 			j := j + 1;
 		}
-		*/
 		i := i + 1;
 	}
-	assert forall i, j :: 0 <= i < n && 0 <= j < n ==> mat[i,j];
+}
+predicate INV(mat: array2<bool>, i: int)
+	requires mat != null
+	requires 0 <= i < mat.Length0
+{
+	forall j :: 0 <= j < mat.Length1 ==> mat[i,j]
 }
